add type inference to untyped->typed translation
@ insert subtyping in the type system

Mica/TinyML/Typed.lean
@@ -5,33 +5,53 @@ namespace Typed
 
 open TinyML
 
-inductive Binder where
-  | none
-  | named (name : Var) (ty : Option Typ)
-  deriving Repr, Inhabited, DecidableEq
+structure Binder where
+  name : Option Var
+  ty : Typ
+  deriving Repr
+
+instance : Inhabited Binder := ⟨⟨Option.none, .value⟩⟩
+
+instance : DecidableEq Binder := by
+  intro a b
+  cases a with
+  | mk n1 t1 =>
+    cases b with
+    | mk n2 t2 =>
+      exact match decEq n1 n2, decEq t1 t2 with
+        | isTrue h1, isTrue h2 => isTrue (by subst h1; subst h2; rfl)
+        | isFalse h, _ => isFalse (by intro heq; cases heq; exact h rfl)
+        | _, isFalse h => isFalse (by intro heq; cases heq; exact h rfl)
+
+def Binder.none (ty : Typ) : Binder := ⟨Option.none, ty⟩
+
+def Binder.named (name : Var) (ty : Typ) : Binder := ⟨some name, ty⟩
 
 instance : BEq Binder := ⟨fun a b => decide (a = b)⟩
 
 instance : LawfulBEq Binder where
-  eq_of_beq h := of_decide_eq_true h
-  rfl := by simp [BEq.beq]
+  eq_of_beq {a b} h := by
+    exact of_decide_eq_true h
+  rfl {a} := by
+    simp [BEq.beq]
 
 inductive Expr where
   | const (c : Const)
-  | var (name : Var)
-  | unop (op : UnOp) (e : Expr)
-  | binop (op : BinOp) (lhs rhs : Expr)
-  | fix (self : Binder) (args : List Binder) (retTy : Option Typ) (body : Expr)
-  | app (fn : Expr) (args : List Expr)
-  | ifThenElse (cond thn els : Expr)
+  | var (name : Var) (ty : Typ)
+  | unop (op : UnOp) (e : Expr) (ty : Typ)
+  | binop (op : BinOp) (lhs rhs : Expr) (ty : Typ)
+  | fix (self : Binder) (args : List Binder) (retTy : Typ) (body : Expr)
+  | app (fn : Expr) (args : List Expr) (ty : Typ)
+  | ifThenElse (cond thn els : Expr) (ty : Typ)
   | letIn (name : Binder) (bound body : Expr)
   | ref    (e : Expr)
-  | deref  (e : Expr)
+  | deref  (e : Expr) (ty : Typ)
   | store  (loc val : Expr)
   | assert (e : Expr)
   | tuple (es : List Expr)
   | inj (tag : Nat) (arity : Nat) (payload : Expr)
-  | match_ (scrutinee : Expr) (branches : List (Binder × Expr))
+  | match_ (scrutinee : Expr) (branches : List (Binder × Expr)) (ty : Typ)
+  | cast (e : Expr) (ty : Typ)
 
 instance : Inhabited Expr := ⟨.const .unit⟩
 
@@ -47,7 +67,6 @@ theorem Expr.isFunc_elim {e : Expr} (h : e.isFunc = true) :
   cases e <;> simp [isFunc] at h
   exact ⟨_, _, _, _, rfl⟩
 
-
 mutual
   def Expr.decEq (a b : Expr) : Decidable (a = b) := by
     cases a <;> cases b
@@ -56,18 +75,24 @@ mutual
     case const.const c1 c2 => exact match decEq c1 c2 with
       | isTrue h => isTrue (by subst h; rfl)
       | isFalse h => isFalse (by intro heq; cases heq; exact h rfl)
-    case var.var n1 n2 => exact match decEq n1 n2 with
-      | isTrue h => isTrue (by subst h; rfl)
-      | isFalse h => isFalse (by intro heq; cases heq; exact h rfl)
-    case unop.unop o1 e1 o2 e2 => exact match decEq o1 o2, e1.decEq e2 with
+    case var.var n1 t1 n2 t2 => exact match decEq n1 n2, decEq t1 t2 with
       | isTrue h1, isTrue h2 => isTrue (by subst h1; subst h2; rfl)
       | isFalse h, _ => isFalse (by intro heq; cases heq; exact h rfl)
       | _, isFalse h => isFalse (by intro heq; cases heq; exact h rfl)
-    case binop.binop o1 l1 r1 o2 l2 r2 => exact match decEq o1 o2, l1.decEq l2, r1.decEq r2 with
+    case unop.unop o1 e1 t1 o2 e2 t2 =>
+      exact match decEq o1 o2, e1.decEq e2, decEq t1 t2 with
       | isTrue h1, isTrue h2, isTrue h3 => isTrue (by subst h1; subst h2; subst h3; rfl)
       | isFalse h, _, _ => isFalse (by intro heq; cases heq; exact h rfl)
       | _, isFalse h, _ => isFalse (by intro heq; cases heq; exact h rfl)
       | _, _, isFalse h => isFalse (by intro heq; cases heq; exact h rfl)
+    case binop.binop o1 l1 r1 t1 o2 l2 r2 t2 =>
+      exact match decEq o1 o2, l1.decEq l2, r1.decEq r2, decEq t1 t2 with
+      | isTrue h1, isTrue h2, isTrue h3, isTrue h4 =>
+        isTrue (by subst h1; subst h2; subst h3; subst h4; rfl)
+      | isFalse h, _, _, _ => isFalse (by intro heq; cases heq; exact h rfl)
+      | _, isFalse h, _, _ => isFalse (by intro heq; cases heq; exact h rfl)
+      | _, _, isFalse h, _ => isFalse (by intro heq; cases heq; exact h rfl)
+      | _, _, _, isFalse h => isFalse (by intro heq; cases heq; exact h rfl)
     case fix.fix s1 args1 rt1 b1 s2 args2 rt2 b2 =>
       exact match decEq s1 s2, decEq args1 args2, decEq rt1 rt2, b1.decEq b2 with
       | isTrue h1, isTrue h2, isTrue h3, isTrue h4 =>
@@ -76,16 +101,20 @@ mutual
       | _, isFalse h, _, _ => isFalse (by intro heq; cases heq; exact h rfl)
       | _, _, isFalse h, _ => isFalse (by intro heq; cases heq; exact h rfl)
       | _, _, _, isFalse h => isFalse (by intro heq; cases heq; exact h rfl)
-    case app.app f1 args1 f2 args2 => exact match f1.decEq f2, exprsDecEq args1 args2 with
-      | isTrue h1, isTrue h2 => isTrue (by subst h1; subst h2; rfl)
-      | isFalse h, _ => isFalse (by intro heq; cases heq; exact h rfl)
-      | _, isFalse h => isFalse (by intro heq; cases heq; exact h rfl)
-    case ifThenElse.ifThenElse c1 t1 e1 c2 t2 e2 =>
-      exact match c1.decEq c2, t1.decEq t2, e1.decEq e2 with
+    case app.app f1 args1 t1 f2 args2 t2 =>
+      exact match f1.decEq f2, exprsDecEq args1 args2, decEq t1 t2 with
       | isTrue h1, isTrue h2, isTrue h3 => isTrue (by subst h1; subst h2; subst h3; rfl)
       | isFalse h, _, _ => isFalse (by intro heq; cases heq; exact h rfl)
       | _, isFalse h, _ => isFalse (by intro heq; cases heq; exact h rfl)
       | _, _, isFalse h => isFalse (by intro heq; cases heq; exact h rfl)
+    case ifThenElse.ifThenElse c1 t1 e1 ty1 c2 t2 e2 ty2 =>
+      exact match c1.decEq c2, t1.decEq t2, e1.decEq e2, decEq ty1 ty2 with
+      | isTrue h1, isTrue h2, isTrue h3, isTrue h4 =>
+        isTrue (by subst h1; subst h2; subst h3; subst h4; rfl)
+      | isFalse h, _, _, _ => isFalse (by intro heq; cases heq; exact h rfl)
+      | _, isFalse h, _, _ => isFalse (by intro heq; cases heq; exact h rfl)
+      | _, _, isFalse h, _ => isFalse (by intro heq; cases heq; exact h rfl)
+      | _, _, _, isFalse h => isFalse (by intro heq; cases heq; exact h rfl)
     case letIn.letIn b1 d1 y1 b2 d2 y2 => exact match decEq b1 b2, d1.decEq d2, y1.decEq y2 with
       | isTrue h1, isTrue h2, isTrue h3 => isTrue (by subst h1; subst h2; subst h3; rfl)
       | isFalse h, _, _ => isFalse (by intro heq; cases heq; exact h rfl)
@@ -94,9 +123,10 @@ mutual
     case ref.ref e1 e2 => exact match e1.decEq e2 with
       | isTrue h => isTrue (by subst h; rfl)
       | isFalse h => isFalse (by intro heq; cases heq; exact h rfl)
-    case deref.deref e1 e2 => exact match e1.decEq e2 with
-      | isTrue h => isTrue (by subst h; rfl)
-      | isFalse h => isFalse (by intro heq; cases heq; exact h rfl)
+    case deref.deref e1 t1 e2 t2 => exact match e1.decEq e2, decEq t1 t2 with
+      | isTrue h1, isTrue h2 => isTrue (by subst h1; subst h2; rfl)
+      | isFalse h, _ => isFalse (by intro heq; cases heq; exact h rfl)
+      | _, isFalse h => isFalse (by intro heq; cases heq; exact h rfl)
     case store.store l1 v1 l2 v2 => exact match l1.decEq l2, v1.decEq v2 with
       | isTrue h1, isTrue h2 => isTrue (by subst h1; subst h2; rfl)
       | isFalse h, _ => isFalse (by intro heq; cases heq; exact h rfl)
@@ -113,7 +143,13 @@ mutual
       | isFalse h, _, _ => isFalse (by intro heq; cases heq; exact h rfl)
       | _, isFalse h, _ => isFalse (by intro heq; cases heq; exact h rfl)
       | _, _, isFalse h => isFalse (by intro heq; cases heq; exact h rfl)
-    case match_.match_ s1 bs1 s2 bs2 => exact match s1.decEq s2, branchesDecEq bs1 bs2 with
+    case match_.match_ s1 bs1 t1 s2 bs2 t2 =>
+      exact match s1.decEq s2, branchesDecEq bs1 bs2, decEq t1 t2 with
+      | isTrue h1, isTrue h2, isTrue h3 => isTrue (by subst h1; subst h2; subst h3; rfl)
+      | isFalse h, _, _ => isFalse (by intro heq; cases heq; exact h rfl)
+      | _, isFalse h, _ => isFalse (by intro heq; cases heq; exact h rfl)
+      | _, _, isFalse h => isFalse (by intro heq; cases heq; exact h rfl)
+    case cast.cast e1 t1 e2 t2 => exact match e1.decEq e2, decEq t1 t2 with
       | isTrue h1, isTrue h2 => isTrue (by subst h1; subst h2; rfl)
       | isFalse h, _ => isFalse (by intro heq; cases heq; exact h rfl)
       | _, isFalse h => isFalse (by intro heq; cases heq; exact h rfl)
@@ -152,62 +188,44 @@ abbrev Vars := List Var
 abbrev Exprs := List Expr
 abbrev Binders := List Binder
 
-@[simp] theorem Binder.named_beq (x z : Var) (tx tz : Option Typ) :
-    (Binder.named x tx == Binder.named z tz) = (x == z && tx == tz) := by
-  apply Bool.eq_iff_iff.mpr
-  simp only [BEq.beq, Bool.and_eq_true, Binder.named.injEq, decide_eq_true_iff]
-  exact and_congr Iff.rfl beq_iff_eq.symm
+def Const.ty : Const → Typ
+  | .int _ => .int
+  | .bool _ => .bool
+  | .unit => .unit
+
+def arrowOfArgs : List Binder → Typ → Typ
+  | [], retTy => retTy
+  | arg :: args, retTy => .arrow arg.ty (arrowOfArgs args retTy)
+
+def Expr.ty : Expr → Typ
+  | .const c => Const.ty c
+  | .var _ ty => ty
+  | .unop _ _ ty => ty
+  | .binop _ _ _ ty => ty
+  | .fix _ args retTy _ => arrowOfArgs args retTy
+  | .app _ _ ty => ty
+  | .ifThenElse _ _ _ ty => ty
+  | .letIn _ _ body => body.ty
+  | .ref e => .ref e.ty
+  | .deref _ ty => ty
+  | .store _ _ => .unit
+  | .assert _ => .unit
+  | .tuple es => .tuple (es.map Expr.ty)
+  | .inj tag arity e => .sum ((List.replicate arity .empty).set tag e.ty)
+  | .match_ _ _ ty => ty
+  | .cast _ ty => ty
 
 structure Decl (S : Type) where
   name : Binder
   body : Expr
   spec : Option S
-  deriving Repr, BEq, Inhabited
+  deriving Repr, BEq
+
+instance [Inhabited S] : Inhabited (Decl S) := ⟨{ name := default, body := default, spec := default }⟩
 
 def Decl.mapSpec {S T : Type} (f : S → Option T) (d : Decl S) : Decl T :=
   { name := d.name, body := d.body, spec := d.spec.bind f }
 
 abbrev Program (S : Type) := List (Decl S)
-
-/-! ### Trivial elaboration from Untyped to Typed -/
-
-def Binder.elaborate : Untyped.Binder → Typed.Binder
-  | .none => .none
-  | .named x ty => .named x ty
-
-mutual
-  def Expr.elaborate : Untyped.Expr → Typed.Expr
-    | .const c => .const c
-    | .var x => .var x
-    | .unop op e => .unop op (Expr.elaborate e)
-    | .binop op l r => .binop op (Expr.elaborate l) (Expr.elaborate r)
-    | .fix self args retTy body =>
-        .fix (Binder.elaborate self) (args.map Binder.elaborate) retTy (Expr.elaborate body)
-    | .app fn args => .app (Expr.elaborate fn) (Exprs.elaborate args)
-    | .ifThenElse c t e => .ifThenElse (Expr.elaborate c) (Expr.elaborate t) (Expr.elaborate e)
-    | .letIn b bound body =>
-        .letIn (Binder.elaborate b) (Expr.elaborate bound) (Expr.elaborate body)
-    | .ref e => .ref (Expr.elaborate e)
-    | .deref e => .deref (Expr.elaborate e)
-    | .store loc val => .store (Expr.elaborate loc) (Expr.elaborate val)
-    | .assert e => .assert (Expr.elaborate e)
-    | .tuple es => .tuple (Exprs.elaborate es)
-    | .inj tag arity payload => .inj tag arity (Expr.elaborate payload)
-    | .match_ scrut branches =>
-        .match_ (Expr.elaborate scrut) (Branches.elaborate branches)
-
-  def Exprs.elaborate : List Untyped.Expr → List Typed.Expr
-    | [] => []
-    | e :: es => Expr.elaborate e :: Exprs.elaborate es
-
-  def Branches.elaborate : List (Untyped.Binder × Untyped.Expr) → List (Typed.Binder × Typed.Expr)
-    | [] => []
-    | (b, e) :: rest => (Binder.elaborate b, Expr.elaborate e) :: Branches.elaborate rest
-end
-def Decl.elaborate {S : Type} (d : Untyped.Decl S) : Typed.Decl S :=
-  { name := Binder.elaborate d.name, body := Expr.elaborate d.body, spec := d.spec }
-
-def Program.elaborate {S : Type} (prog : Untyped.Program S) : Typed.Program S :=
-  prog.map Decl.elaborate
 
 end Typed
